temporary workaround for #352

src/Experiments/SimplyTypedArithmetic.v
@@ -5009,7 +5009,7 @@ Module Compilers.
                      | Some x, Some y, Some z
                        => type.option.Some
                             (t:=(type.Z*type.Z)%ctype)
-                            (let b := ZRange.split_bounds (ZRange.eight_corners (fun x y z => (x - y - z)%Z) x y z) split_at in
+                            (let b := ZRange.split_bounds (ZRange.eight_corners (fun x y z => (y - z - x)%Z) x y z) split_at in
                              (* N.B. sub_get_borrow returns - ((x - y) / split_at) as the borrow, so we need to negate *)
                                (fst b, ZRange.opp (snd b)))
                      | _, _, _ => type.option.None
@@ -7631,6 +7631,7 @@ Module PrintingNotations.
   Notation "'ADDC_256' ( x ,  y ,  z )" := (ident.Z.cast2 (uint256, bool)%core @@ (ident.Z.add_with_get_carry_concrete TwoPow256 @@ (x, y, z)))%expr : expr_scope.
   Notation "'ADDC_128' ( x ,  y ,  z )" := (ident.Z.cast2 (uint128, bool)%core @@ (ident.Z.add_with_get_carry_concrete TwoPow256 @@ (x, y, z)))%expr : expr_scope.
   Notation "'SUB_256' ( x ,  y )" := (ident.Z.cast2 (uint256, bool)%core @@ (ident.Z.sub_get_borrow_concrete TwoPow256 @@ (x, y)))%expr : expr_scope.
+  Notation "'SUBB_256' ( x ,  y , z )" := (ident.Z.cast2 (uint256, bool)%core @@ (ident.Z.sub_with_get_borrow_concrete TwoPow256 @@ (x, y, z)))%expr : expr_scope.
   Notation "'ADDM' ( x ,  y ,  z )" := (ident.Z.cast uint256 @@ (ident.Z.add_modulo @@ (x, y, z)))%expr : expr_scope.
   Notation "'RSHI' ( x ,  y ,  z )" := (ident.Z.cast _ @@ (ident.Z.rshi_concrete _ z @@ (x, y)))%expr : expr_scope.
   Notation "'SELC' ( x ,  y ,  z )" := (ident.Z.cast uint256 @@ (ident.Z.zselect @@ (x, y, z)))%expr : expr_scope.
@@ -8614,6 +8615,7 @@ Module PreFancy.
       | add (imm : BinInt.Z) : ident (Z * Z) (Z * Z)
       | addc (imm : BinInt.Z) : ident (Z * Z * Z) (Z * Z)
       | sub (imm : BinInt.Z) : ident (Z * Z) (Z * Z)
+      | subb (imm : BinInt.Z) : ident (Z * Z * Z) (Z * Z)
       | mulll : ident (Z * Z) Z
       | mullh : ident (Z * Z) Z
       | mulhl : ident (Z * Z) Z
@@ -8774,6 +8776,19 @@ Module PreFancy.
               | _ => dummy _
               end
             else dummy _
+        | ident.Z.sub_with_get_borrow_concrete w =>
+          fun t r x f =>
+            if w =? wordmax
+            then
+              match x with
+              | Pair (type.prod Z Z) Z (Pair Z Z xb xl) xr =>
+                match invert_shift xr with
+                | Some (xr', imm) => LetInAppIdentZZ r (subb imm) (Pair (Pair xb xl) xr') f
+                | None => LetInAppIdentZZ r (subb 0) (Pair (Pair xb xl) xr) f
+                end
+              | _ => dummy _
+              end
+            else dummy _
         | ident.Z.rshi_concrete w n =>
           fun _ r x f =>
             if w =? wordmax
@@ -8840,6 +8855,7 @@ Module PreFancy.
         | add imm => fun x => Z.add_get_carry_full wordmax (fst x) (shift (snd x) imm)
         | addc imm => fun x => Z.add_with_get_carry_full wordmax (fst (fst x)) (snd (fst x)) (shift (snd x) imm)
         | sub imm => fun x => Z.sub_get_borrow_full wordmax (fst x) (shift (snd x) imm)
+        | subb imm => fun x => Z.sub_with_get_borrow_full wordmax (fst (fst x)) (snd (fst x)) (shift (snd x) imm)
         | mulll => fun x => low (fst x) * low (snd x)
         | mullh => fun x => low (fst x) * high (snd x)
         | mulhl => fun x => high (fst x) * low (snd x)
@@ -8990,6 +9006,16 @@ Module PreFancy.
                      (Pair x y)
                      (word_range, flag_range)
                      (ident.Z.sub_get_borrow_concrete wordmax)
+      | ok_subb :
+          forall b x y : scalar type.Z,
+            in_flag_range (get_range b) ->
+            in_word_range (get_range x) ->
+            in_word_range (get_range y) ->
+            ok_ident _
+                     (type.prod type.Z type.Z)
+                     (Pair (Pair b x) y)
+                     (word_range, flag_range)
+                     (ident.Z.sub_with_get_borrow_concrete wordmax)
       | ok_rshi :
           forall (x : scalar (type.prod type.Z type.Z)) n,
             in_word_range (fst (get_range x)) ->
@@ -9397,6 +9423,12 @@ Module PreFancy.
           match goal with |- context[?x mod ?m] => pose proof (Z.mod_pos_bound x m ltac:(omega)) end.
           rewrite Z.div_sub_small by omega.
           split; break_match; lia. }
+        {
+          autorewrite with to_div_mod.
+          match goal with |- context [?a - ?b - ?c] => replace (a - b - c) with (a - (b + c)) by ring end.
+          match goal with |- context[?x mod ?m] => pose proof (Z.mod_pos_bound x m ltac:(omega)) end.
+          rewrite Z.div_sub_small by omega.
+          split; break_match; lia. }
         { apply has_word_range_rshi; omega. }
         { rewrite Z.zselect_correct. break_match; omega. }
         { cbn [interp_scalar fst snd get_range] in *.
@@ -9793,6 +9825,9 @@ Module PreFancy.
     Notation "sub@( y , x1 , x2 , n ); g"
       := (LetInAppIdentZZ (uint256, bool) (sub n) (Pair x1 x2) (fun y => g))
            (at level 10, g at level 200, format "sub@( y ,  x1 ,  x2 ,  n ); '//' g").
+    Notation "subb@( y , x1 , x2 , x3 , n ); g"
+      := (LetInAppIdentZZ (uint256, bool) (subb n) (Pair (Pair x1 x2) x3) (fun y => g))
+           (at level 10, g at level 200, format "subb@( y ,  x1 ,  x2 ,  x3 ,  n ); '//' g").
     Notation "rshi@( y , x1 , x2 , n ); g"
       := (LetInAppIdentZ _ (rshi n) (Pair x1 x2) (fun y => g))
            (at level 10, g at level 200, format "rshi@( y ,  x1 ,  x2 , n ); '//' g ").
@@ -9926,6 +9961,15 @@ Module Fancy.
         spec := (fun '(r0, r1) cc =>
                    r0 - (r1 << imm))
       |}.
+
+    Definition SUBC (imm : int) : instruction :=
+      {|
+        num_source_regs := 2;
+        writes_conditions := [C; M; L; Z];
+        spec := (fun '(r0, r1) cc =>
+                   r0 - (r1 << imm) - cc[C])
+      |}.
+
 
     Definition MUL128LL : instruction :=
       {|
@@ -10093,6 +10137,8 @@ Module Fancy.
                                existT _ (ADDC imm) (of_prefancy_scalar (Pair (Snd (Fst args)) (Snd args)))
       | PreFancy.sub imm => fun args : @scalar var (type.Z * type.Z) =>
                               existT _ (SUB imm) (of_prefancy_scalar args)
+      | PreFancy.subb imm => fun args : @scalar var (type.Z * type.Z * type.Z) =>
+                               existT _ (SUBC imm) (of_prefancy_scalar (Pair (Snd (Fst args)) (Snd args)))
       | PreFancy.mulll => fun args : @scalar var (type.Z * type.Z) =>
                             existT _ MUL128LL (of_prefancy_scalar args)
       | PreFancy.mullh => fun args : @scalar var (type.Z * type.Z) =>
@@ -10514,7 +10560,7 @@ Module BarrettReduction.
       dlet_nd qt := qt in
       dlet_nd r2 := mul (low qt) M in
       dlet_nd r := sub xt r2 in
-      dlet_nd q3 := cond_sub1 r M in
+      let q3 := cond_sub1 r M in
       cond_sub2 q3 M.
 
     Lemma looser_bound : M * 2 ^ k < 2 ^ (2*k).
@@ -10698,7 +10744,16 @@ Module BarrettReduction.
     Ltac change_weight := rewrite !Hw, ?Z.pow_0_r, ?Z.pow_1_r, ?Z.pow_2_r.
 
     Definition wideadd t1 t2 := fst (Rows.add w 2 t1 t2).
-    Definition widesub t1 t2 := fst (Rows.sub w 2 t1 t2).
+    (* TODO: use this definition once issue #352 is resolved *)
+    (* Definition widesub t1 t2 := fst (Rows.sub w 2 t1 t2). *)
+    Definition widesub (t1 t2 : list Z) :=
+      let t1_0 := hd 0 t1 in
+      let t1_1 := hd 0 (tl t1) in
+      let t2_0 := hd 0 t2 in
+      let t2_1 := hd 0 (tl t2) in
+      dlet_nd x0 := Z.sub_get_borrow_full (2^k) t1_0 t2_0 in
+      dlet_nd x1 := Z.sub_with_get_borrow_full (2^k) (snd x0) t1_1 t2_1 in
+      [fst x0; fst x1].
     Definition widemul := BaseConversion.widemul_inlined k n nout.
 
     Lemma partition_represents x :
@@ -10739,7 +10794,27 @@ Module BarrettReduction.
       represents t2 y ->
       0 <= x - y < 2^k*2^k ->
       represents (widesub t1 t2) (x - y).
+    Proof.
+      intros; cbv [widesub Let_In].
+      rewrite (represents_eq t1 x) by assumption.
+      rewrite (represents_eq t2 y) by assumption.
+      cbn [hd tl].
+      autorewrite with to_div_mod.
+      pull_Zmod.
+      match goal with |- represents [?m; ?d] ?x =>
+                      replace d with (x / 2 ^ k); [solve [auto using represents_id] |] end.
+      rewrite <-(Z.mod_small ((x - y) / 2^k) (2^k)) by (split; try apply Z.div_lt_upper_bound; Z.zero_bounds).
+      f_equal.
+      transitivity ((x mod 2^k - y mod 2^k + 2^k * (x / 2 ^ k) - 2^k * (y / 2^k)) / 2^k). {
+        rewrite (Z.div_mod x (2^k)) at 1 by auto using Z.pow_nonzero with omega.
+        rewrite (Z.div_mod y (2^k)) at 1 by auto using Z.pow_nonzero with omega.
+        f_equal. ring. }
+      autorewrite with zsimplify.
+      ring.
+    Qed.
+    (* Works with Rows.sub-based widesub definition
     Proof. intros; cbv [widesub]. wide_op Rows.sub_partitions. Qed.
+    *)
 
     Lemma widemul_represents x y :
       0 <= x < 2^k ->
@@ -10836,7 +10911,8 @@ Module BarrettReduction.
 
     Definition cond_sub1 (a : list Z) y : Z :=
       dlet_nd maybe_y := Z.zselect (Z.cc_l (high a)) 0 y in
-      fst (Z.sub_get_borrow_full (2^k) (low a) maybe_y).
+      dlet_nd diff := Z.sub_get_borrow_full (2^k) (low a) maybe_y in
+      fst diff.
 
     Lemma cc_l_only_bit : forall x s, 0 <= x < 2 * s -> Z.cc_l (x / s) = 0 <-> x < s.
     Proof.
@@ -10928,7 +11004,7 @@ Module BarrettReduction.
                       = barrett_reduce k M muLow n nout xLow xHigh)
          As barrett_red_gen_correct.
   Proof. Time cache_reify (). exact admit. (* correctness of initial parts of the pipeline *) Time Qed.
-  (* TODO : reification here is still quite slow (~40s on a beefy machine). Possibly just due to size of term, but warrants further investigation. *)
+  (* TODO : reification here is still quite slow (~90s on a beefy machine). Possibly just due to size of term, but warrants further investigation. *)
   Module Export ReifyHints.
     Global Hint Extern 1 (_ = barrett_reduce _ _ _ _ _ _ _) => simple apply barrett_red_gen_correct : reify_gen_cache.
   End ReifyHints.
@@ -11010,9 +11086,6 @@ Module Barrett256.
   Open Scope expr_scope.
 
   Print barrett_red256.
-  (* TODO: the ADD/ADDC instructions containing Z.opp should be translated to SUB/SUBB in partial evaluation *)
-  (* Note: the aforementioned ADD/ADDC instructions currently *do* fail to bounds-check, although the pipeline doesn't give an error.
-     This is why their results are not cast (because the carry has range [-1~>0]). *)
   (*
 barrett_red256 =  fun var : type -> Type => λ x : var (type.type_primitive type.Z * type.type_primitive type.Z)%ctype,
                 expr_let x0 := SELM (x₂, 0, 26959946667150639793205513449348445388433292963828203772348655992835) in
@@ -11039,11 +11112,11 @@ barrett_red256 =  fun var : type -> Type => λ x : var (type.type_primitive type
                 expr_let x21 := ADDC_256 (x20₂, (uint128)(x18 >> 128), x16) in
                 expr_let x22 := ADD_256 ((uint256)(((uint128)(x17) & 340282366920938463463374607431768211455) << 128), x20₁) in
                 expr_let x23 := ADDC_256 (x22₂, (uint128)(x17 >> 128), x21₁) in
-                expr_let x24 := Z.add_get_carry_concrete 115792089237316195423570985008687907853269984665640564039457584007913129639936 @@ (Z.opp @@ (fst @@ x22), x₁) in
-                expr_let x25 := Z.add_with_get_carry_concrete 115792089237316195423570985008687907853269984665640564039457584007913129639936 @@ (x24₂, Z.opp @@ (fst @@ x23), x₂) in
+                expr_let x24 := SUB_256 (x₁, x22₁) in
+                expr_let x25 := SUBB_256 (x24₂, x₂, x23₁) in
                 expr_let x26 := SELL (x25₁, 0, 115792089210356248762697446949407573530086143415290314195533631308867097853951) in
-                expr_let x27 := Z.cast uint256 @@ (fst @@ SUB_256 (x24₁, x26)) in
-                ADDM (x27, 0, 115792089210356248762697446949407573530086143415290314195533631308867097853951)
+                expr_let x27 := SUB_256 (x24₁, x26) in
+                ADDM (x27₁, 0, 115792089210356248762697446949407573530086143415290314195533631308867097853951)
      : Expr (type.uncurry (type.type_primitive type.Z -> type.type_primitive type.Z -> type.type_primitive type.Z))
   *)
 
@@ -11056,7 +11129,6 @@ barrett_red256 =  fun var : type -> Type => λ x : var (type.type_primitive type
   Local Notation "'RegMod'" := (Straightline.expr.Primitive (t:=type.Z) 115792089210356248762697446949407573530086143415290314195533631308867097853951).
   Local Notation "'RegMuLow'" := (Straightline.expr.Primitive (t:=type.Z) 26959946667150639793205513449348445388433292963828203772348655992835).
   Print barrett_red256_prefancy.
-  (* Note : currently (correctly) fails to convert the adds that should be subs *)
   (*
     selm@(y, $x₂, RegZero, RegMuLow);
     rshi@(y0, RegZero, $x₂,255);
@@ -11081,8 +11153,13 @@ barrett_red256 =  fun var : type -> Type => λ x : var (type.type_primitive type
     add@(y19, $y18, $y17, 128);
     addc@(y20, carry{$y19}, $y15, $y17, -128);
     add@(y21, $y19, $y16, 128);
-    addc@(_, carry{$y21}, $y20, $y16, -128);
-    Straightline.expr.Scalar (Straightline.expr.Primitive (-1))            
+    addc@(y22, carry{$y21}, $y20, $y16, -128);
+    sub@(y23, $x₁, $y21, 0);
+    subb@(y24, carry{$y23}, $x₂, $y22, 0);
+    sell@(y25, $y24, RegZero, RegMod);
+    sub@(y26, $y23, $y25, 0);
+    addm@(y27, $y26, RegZero, RegMod);
+    ret $y27 
   *)
 End Barrett256.
 
